\documentclass{beamer}
\usetheme{metropolis}
\usepackage{graphicx}
\usepackage{amsmath}
\title{Electromagnetc Theory: PHYS330}
\author{Jordan Hanson}
\institute{Whittier College Department of Physics and Astronomy}

\begin{document}
\maketitle

\section{Class Notes}

\begin{frame}{Warm-Up 1}
Suppose we have an electron traveling at 1 percent of the speed of light, with a velocity vector
\begin{equation}
\vec{v} = \frac{|\vec{v}|}{\sqrt{2}} \hat{i} + \frac{|\vec{v}|}{\sqrt{2}} \hat{j}
\end{equation}
The electron is traveling in a $\vec{B}$-field of 0.5 Gauss ($0.5 \times 10^{-4}$ Tesla) that is pointed in the z-direction.  What is the force on the electron?  \textit{[Hint: $\vec{F} = q\vec{v} \times \vec{B}$]}
\end{frame}

\begin{frame}{Answer}
Answers (build up the answer from smaller pieces):
\begin{align}
\vec{v} &= a(\hat{i} + \hat{j}) \\
\vec{B} &= B \hat{k} \\
\vec{v} \times \vec{B} &= a B (\hat{i} \times \hat{k} + \hat{j} \times \hat{k}) \\
\vec{v} \times \vec{B} &= a B (\hat{i} - \hat{j}) \\
\vec{v} \times \vec{B} &= \frac{|\vec{v}|B}{\sqrt{2}} (\hat{i} - \hat{j})
\end{align}
Now, we want to add $q$, and the values of $B$ and $v$ ...
\end{frame}

\begin{frame}{Warm-Up 2}
Suppose we have a function that describes the \textit{potential energy} of a system:
\begin{equation}
U(x,y,z) = m g z
\end{equation}
Take the gradient and multiply by minus one.  What do you get? \textit{[Hint: $\vec{F} = - \nabla U(x,y,z)$.]}
\end{frame}

\begin{frame}{Warm-Up 2}
Answer:
\begin{equation}
-\nabla U(x,y,z) = -\left(\hat{i}\frac{\partial}{\partial x} + \hat{j}\frac{\partial}{\partial y} + \hat{k}\frac{\partial}{\partial z}\right) m g z
\end{equation}
Take the gradient and multiply by minus one.  What do you get? \textit{[Hint: $\vec{F} = - \nabla U(x,y,z)$.]}
\end{frame}

\section{More Class Notes}

\begin{frame}{Gradient of $r = \sqrt{x^2 + y^2  + z^2}$}
\begin{equation}
\nabla r = \left(\hat{i}\frac{\partial r}{\partial x} + \hat{j}\frac{\partial r}{\partial y} + \hat{k}\frac{\partial r}{\partial z}\right)
\end{equation}
(Break the problem into pieces ... )
\begin{align}
\frac{\partial r}{\partial x} &= \frac{\partial }{\partial x} (x^2 + ... )^{1/2} = \frac{1}{2}(x^2 + ... )^{-1/2}(2x) \\
\frac{\partial r}{\partial y} &= \frac{\partial }{\partial y} (y^2 + ... )^{1/2} = \frac{1}{2}(y^2 + ... )^{-1/2}(2y) \\
\frac{\partial r}{\partial z} &= \frac{\partial }{\partial z} (z^2 + ... )^{1/2} = \frac{1}{2}(z^2 + ... )^{-1/2}(2z)
\end{align}
The result is:
\begin{equation}
\nabla r = \hat{r}
\end{equation}
\end{frame}

\end{document}
